week2/problems/problem2.dfy
@@ -3,6 +3,7 @@
 
 method IntegerDivision(dividend: int, divisor: int) returns (quotient: int, remainder: int)
     requires divisor > 0
+    requires dividend >= 0
     ensures dividend == divisor * quotient + remainder
     ensures 0 <= remainder < divisor
 {
@@ -10,7 +11,8 @@ method IntegerDivision(dividend: int, divisor: int) returns (quotient: int, rema
     remainder := dividend;
     
     while remainder >= divisor
-        // TODO: Write loop invariant(s)
+        invariant dividend == divisor * quotient + remainder
+        invariant remainder >= 0
         decreases remainder
     {
         quotient := quotient + 1;
